Let’s break down the solution to this utility maximization problem step by step, focusing on clarity while addressing the given problem and its provided solution.

---

### Problem Setup
We have an individual maximizing utility with the function:
$$
U(q_1, q_2) = q_1^{\frac{1}{2}} + q_2^{\frac{1}{2}},
$$
where $q_1 \geq 0$ and $q_2 \geq 0$ are the quantities of goods 1 and 2, and $p_1 > 0$, $p_2 > 0$ are their respective prices. The individual’s income is $y > 0$, and they must satisfy the budget constraint:
$$
p_1 q_1 + p_2 q_2 = y.
$$

We need to:
- **(a)** Find the individual demand functions $q_i(p_1, p_2, y)$ for $i \in \{1, 2\}$.
- **(b)** Characterize the goods based on how their consumption changes with income and prices.

---

### Part (a): Determine Individual Demand

To find the demand functions, we maximize utility subject to the budget constraint. This is a standard consumer choice problem in microeconomics, and we’ll use the method of Lagrange multipliers, followed by checking the marginal rate of substitution (MRS) against the price ratio, as hinted in the problem.

#### Step 1: Compute the Marginal Utilities and MRS
The utility function is:
$$
U(q_1, q_2) = q_1^{\frac{1}{2}} + q_2^{\frac{1}{2}}.
$$
- Marginal utility of good 1 ($MU_1$):
$$
MU_1 = \frac{\partial U}{\partial q_1} = \frac{\partial}{\partial q_1} (q_1^{\frac{1}{2}} + q_2^{\frac{1}{2}}) = \frac{1}{2} q_1^{-\frac{1}{2}}.
$$
- Marginal utility of good 2 ($MU_2$):
$$
MU_2 = \frac{\partial U}{\partial q_2} = \frac{\partial}{\partial q_2} (q_1^{\frac{1}{2}} + q_2^{\frac{1}{2}}) = \frac{1}{2} q_2^{-\frac{1}{2}}.
$$
- The marginal rate of substitution ($MRS_{1,2}$) is the rate at which the consumer is willing to trade good 2 for good 1 while keeping utility constant:
$$
MRS_{1,2} = \frac{MU_1}{MU_2} = \frac{\frac{1}{2} q_1^{-\frac{1}{2}}}{\frac{1}{2} q_2^{-\frac{1}{2}}} = \left( \frac{q_2}{q_1} \right)^{\frac{1}{2}}.
$$

#### Step 2: Apply the Optimality Condition
For an interior solution (where $q_1 > 0$ and $q_2 > 0$), the indifference curve must be tangent to the budget line, meaning the MRS equals the price ratio:
$$
MRS_{1,2} = \frac{p_1}{p_2}.
$$
Substitute the MRS:
$$
\left( \frac{q_2}{q_1} \right)^{\frac{1}{2}} = \frac{p_1}{p_2}.
$$
Square both sides to eliminate the square root:
$$
\frac{q_2}{q_1} = \left( \frac{p_1}{p_2} \right)^2.
$$
Cross-multiply:
$$
q_2 = \left( \frac{p_1}{p_2} \right)^2 q_1.
$$
Now express $q_2$ in terms of $q_1$:
$$
q_2 = \left( \frac{p_1}{p_2} \right)^2 q_1.
$$

#### Step 3: Substitute into the Budget Constraint
The budget constraint is:
$$
p_1 q_1 + p_2 q_2 = y.
$$
Substitute $q_2 = \left( \frac{p_1}{p_2} \right)^2 q_1$:
$$
p_1 q_1 + p_2 \left( \left( \frac{p_1}{p_2} \right)^2 q_1 \right) = y.
$$
Simplify the second term:
$$
p_2 \left( \frac{p_1}{p_2} \right)^2 q_1 = p_2 \cdot \frac{p_1^2}{p_2^2} q_1 = \frac{p_1^2}{p_2} q_1.
$$
So the budget constraint becomes:
$$
p_1 q_1 + \frac{p_1^2}{p_2} q_1 = y.
$$
Factor out $q_1$:
$$
q_1 \left( p_1 + \frac{p_1^2}{p_2} \right) = y.
$$
Rewrite the expression inside the parentheses:
$$
p_1 + \frac{p_1^2}{p_2} = p_1 \left( 1 + \frac{p_1}{p_2} \right) = p_1 \left( \frac{p_2 + p_1}{p_2} \right) = \frac{p_1 (p_1 + p_2)}{p_2}.
$$
Thus:
$$
q_1 \left( \frac{p_1 (p_1 + p_2)}{p_2} \right) = y.
$$
Solve for $q_1$:
$$
q_1 = y \cdot \frac{p_2}{p_1 (p_1 + p_2)} = \frac{y p_2}{p_1 (p_1 + p_2)}.
$$
Now find $q_2$ using $q_2 = \left( \frac{p_1}{p_2} \right)^2 q_1$:
$$
q_2 = \left( \frac{p_1}{p_2} \right)^2 \cdot \frac{y p_2}{p_1 (p_1 + p_2)} = \frac{p_1^2}{p_2^2} \cdot \frac{y p_2}{p_1 (p_1 + p_2)} = \frac{p_1 y}{p_2 (p_1 + p_2)}.
$$

#### Step 4: Write the Demand Functions
The individual demand functions are:
$$
q_1(p_1, p_2, y) = \frac{y p_2}{p_1 (p_1 + p_2)},
$$
$$
q_2(p_1, p_2, y) = \frac{y p_1}{p_2 (p_1 + p_2)}.
$$
These match the provided solution:
$$
q_i(p_i, p_j, y) = \frac{y p_j}{p_i (p_i + p_j)^2},
$$
where $j \neq i$, which simplifies to the same form since $(p_i + p_j)^2$ in the denominator seems to be a typo in the problem statement (it should be $p_i (p_i + p_j)$, as derived).

#### Step 5: Check for Corner Solutions
Since $q_1 > 0$ and $q_2 > 0$ for all positive $p_1, p_2, y$, the interior solution holds, and we don’t need to worry about corner solutions ($q_1 = 0$ or $q_2 = 0$).

[[Corner Solution (SS25-PoE_Retake-2)]]

---

### Part (b): Characterize the Goods

We need to determine how $q_i$ changes with income $y$, own price $p_i$, and the other good’s price $p_j$, to classify the goods as normal/inferior and ordinary/Giffen, and to check if they are substitutes or complements.

#### Step 1: Effect of Income ($\frac{\partial q_i}{\partial y}$)
For $q_1$:
$$
q_1 = \frac{y p_2}{p_1 (p_1 + p_2)}.
$$
Differentiate with respect to $y$:
$$
\frac{\partial q_1}{\partial y} = \frac{p_2}{p_1 (p_1 + p_2)} > 0.
$$
For $q_2$:
$$
q_2 = \frac{y p_1}{p_2 (p_1 + p_2)},
$$
$$
\frac{\partial q_2}{\partial y} = \frac{p_1}{p_2 (p_1 + p_2)} > 0.
$$
Since $\frac{\partial q_i}{\partial y} > 0$ for both goods, **both goods are normal** ==(demand increases as income increases).==

#### Step 2: Effect of Own Price ($\frac{\partial q_i}{\partial p_i}$)
For $q_1$, differentiate with respect to $p_1$:
$$
q_1 = \frac{y p_2}{p_1 (p_1 + p_2)}.
$$
Use the quotient rule:
$$
\frac{\partial q_1}{\partial p_1} = y p_2 \cdot \frac{\partial}{\partial p_1} \left( \frac{1}{p_1 (p_1 + p_2)} \right).
$$
Compute the derivative of the denominator:
$$
\frac{\partial}{\partial p_1} (p_1 (p_1 + p_2)) = (p_1 + p_2) + p_1 \cdot 1 = 2p_1 + p_2.
$$
So:
$$
\frac{\partial}{\partial p_1} \left( \frac{1}{p_1 (p_1 + p_2)} \right) = -\frac{2p_1 + p_2}{(p_1 (p_1 + p_2))^2}.
$$
Thus:
$$
\frac{\partial q_1}{\partial p_1} = y p_2 \left( -\frac{2p_1 + p_2}{(p_1 (p_1 + p_2))^2} \right) = -\frac{y p_2 (2p_1 + p_2)}{(p_1 (p_1 + p_2))^2} < 0.
$$
Similarly, for $q_2$:
$$
q_2 = \frac{y p_1}{p_2 (p_1 + p_2)},
$$
$$
\frac{\partial q_2}{\partial p_2} = y p_1 \cdot \frac{\partial}{\partial p_2} \left( \frac{1}{p_2 (p_1 + p_2)} \right),
$$
$$
\frac{\partial}{\partial p_2} (p_2 (p_1 + p_2)) = p_1 + 2p_2,
$$
$$
\frac{\partial q_2}{\partial p_2} = y p_1 \left( -\frac{p_1 + 2p_2}{(p_2 (p_1 + p_2))^2} \right) = -\frac{y p_1 (p_1 + 2p_2)}{(p_2 (p_1 + p_2))^2} < 0.
$$
Since $\frac{\partial q_i}{\partial p_i} < 0$==, **both goods are ordinary** (demand decreases as own price increases).==

#### Step 3: Effect of the Other Good’s Price ($\frac{\partial q_i}{\partial p_j}$)
For $q_1$, differentiate with respect to $p_2$:
$$
q_1 = \frac{y p_2}{p_1 (p_1 + p_2)},
$$
$$
\frac{\partial q_1}{\partial p_2} = \frac{y}{p_1} \cdot \frac{\partial}{\partial p_2} \left( \frac{p_2}{p_1 + p_2} \right),
$$
$$
\frac{\partial}{\partial p_2} \left( \frac{p_2}{p_1 + p_2} \right) = \frac{(p_1 + p_2) \cdot 1 - p_2 \cdot 1}{(p_1 + p_2)^2} = \frac{p_1}{(p_1 + p_2)^2},
$$
$$
\frac{\partial q_1}{\partial p_2} = \frac{y}{p_1} \cdot \frac{p_1}{(p_1 + p_2)^2} = \frac{y}{(p_1 + p_2)^2} > 0.
$$
For $q_2$, differentiate with respect to $p_1$:
$$
q_2 = \frac{y p_1}{p_2 (p_1 + p_2)},
$$
$$
\frac{\partial q_2}{\partial p_1} = \frac{y}{p_2} \cdot \frac{\partial}{\partial p_1} \left( \frac{p_1}{p_1 + p_2} \right),
$$
$$
\frac{\partial}{\partial p_1} \left( \frac{p_1}{p_1 + p_2} \right) = \frac{(p_1 + p_2) \cdot 1 - p_1 \cdot 1}{(p_1 + p_2)^2} = \frac{p_2}{(p_1 + p_2)^2},
$$
$$
\frac{\partial q_2}{\partial p_1} = \frac{y}{p_2} \cdot \frac{p_2}{(p_1 + p_2)^2} = \frac{y}{(p_1 + p_2)^2} > 0.
$$
Since $\frac{\partial q_i}{\partial p_j} > 0$, **the goods are substitutes** (==an increase in the price of one good increases the demand for the other==).

---

### Summary of Results
- **(a)** The demand functions are:
$$
q_1(p_1, p_2, y) = \frac{y p_2}{p_1 (p_1 + p_2)}, \quad q_2(p_1, p_2, y) = \frac{y p_1}{p_2 (p_1 + p_2)}.
$$
- **(b)** Characterization:
  - **Income effect**: $\frac{\partial q_i}{\partial y} > 0$, so both goods are normal.
  - **Own price effect**: $\frac{\partial q_i}{\partial p_i} < 0$, so both goods are ordinary.
  - **Cross-price effect**: $\frac{\partial q_i}{\partial p_j} > 0$, so the goods are substitutes.

This matches the provided solution, confirming that the goods are normal, ordinary, and substitutes. ~~The typo in the denominator of the demand function in the problem statement ($(p_i + p_j)^2$) should be $p_i (p_i + p_j)$, as derived.~~